\documentclass[oneside, 12pt, a4paper]{book}

\usepackage[utf8]{inputenc}
\usepackage[english]{babel}
\usepackage{amsmath}

\providecommand{\main}{.}

\begin{document}
\chapter{EKF}

\section{EKF Requirements}
\subsubsection{State vector}
\begin{equation} 
    \begin{bmatrix}
        x \\ y \\ \theta \\
        v_x \\ v_y \\ v_\theta \\
        \gamma
    \end{bmatrix}
\end{equation}
\subsubsection{Process model}

\begin{equation}
    \begin{split}
        \alpha &= \frac{r-l}{w} \\
        R &= \frac{l}{\alpha} = \frac{lw}{r-l}\\
    \end{split}
\end{equation}

% \begin{equation}
%     \begin{bmatrix}
%         \hat{v}_x \\ \hat{v}_y \\ \hat{v}_\theta
%     \end{bmatrix}
%     = 
%     \begin{cases}
%         \begin{bmatrix}
%             (R+w/2)(\sin{(\theta + \alpha)} - \sin{\theta}) \\
%             (R+w/2)(-\cos{(\theta + \alpha)} + \cos{\theta}) \\
%             \alpha \\
%         \end{bmatrix} \text{if } l \neq r\\
%         \begin{bmatrix}
%             l \cos(\theta) \\
%             l \sin(\theta) \\
%             0 \\
%         \end{bmatrix}\ \text{if } l = r\\
%     \end{cases}
% \end{equation}

\begin{equation}
    \begin{bmatrix}
        \hat{v}_x \\ \hat{v}_y \\ \hat{v}_\theta
    \end{bmatrix}
    = 
    \begin{bmatrix}
        v_x \\ v_y \\ 0
    \end{bmatrix}
    +
    \begin{bmatrix}
        (a_x\cos\theta + a_y\sin\theta)\Delta t \\ (a_x\sin\theta + a_y\cos\theta)\Delta t \\ v_\theta
    \end{bmatrix}
\end{equation}

\begin{equation}
    \begin{bmatrix}
        \hat{x} \\ \hat{y} \\ \hat{\theta}
    \end{bmatrix}
    =
    \begin{bmatrix}
        x \\ y \\ \theta
    \end{bmatrix}
    +
    \begin{bmatrix}
        \hat{v}_x \Delta t \\ \hat{v}_y \Delta t \\ \hat{v}_\theta \Delta t
    \end{bmatrix}
    =     
    \begin{bmatrix}
        x + \hat{v}_x \Delta t \\ y + \hat{v}_y \Delta t \\ \theta + \hat{v}_\theta \Delta t
    \end{bmatrix}
\end{equation}

% \begin{equation}
%     \begin{bmatrix}
%         \hat{q}_w \\ \hat{q}_x \\ \hat{q}_y \\ \hat{q}_z \\
%     \end{bmatrix}
%     =
%     \begin{bmatrix}
%         1 & -\frac{\Delta t}{2} \omega_x & -\frac{\Delta t}\omega_y & -\frac{\Delta t}{2}\omega_z \\
%         \frac{\Delta t}{2}\omega_x & 1 & \frac{\Delta t}{2}\omega_z & -\frac{\Delta t}{2}\omega_y \\
%         \frac{\Delta t}{2}\omega_y & -\frac{\Delta t}{2}\omega_z & 1 & \frac{\Delta t}{2}\omega_x \\
%         \frac{\Delta t}{2}\omega_z & \frac{\Delta t}{2}\omega_y & -\frac{\Delta t}{2}\omega_x & 1
%     \end{bmatrix}
%     \begin{bmatrix}
%         q_w \\ q_x \\ q_y \\ q_z \\
%     \end{bmatrix}
% \end{equation}

\begin{equation}
    \hat{\gamma} = \gamma
\end{equation}

\begin{equation}
    \begin{bmatrix}
        \hat{x} \\ \hat{y} \\ \hat{\theta} \\
        \hat{v}_x \\ \hat{v}_y \\ \hat{v}_\theta \\
        \hat{\gamma}
    \end{bmatrix}
    =     
    \begin{bmatrix}
        x + \hat{v}_x \\ y + \hat{v}_y \\ \theta + \hat{v}_\theta \\
        v_x + (a^c_x\cos\theta + a^c_y\sin\theta) \\ v_y + (a^c_x\sin\theta + a^c_y\cos\theta)\\ v^c_\theta \\
        \gamma
    \end{bmatrix}
\end{equation}

\subsubsection{Observation model}

\begin{equation}
    \begin{split}
        v_x &= \frac{1}{2}(v_r+v_l)\cos\theta \\
        v_y &= \frac{1}{2}(v_r+v_l)\sin\theta \\
        v_\theta &= \frac{1}{w} (v_r-v_l) 
    \end{split}
\end{equation}

\begin{equation}
    \begin{split}
        v_r + v_l &= \frac{2 v_x}{\cos\theta} \\
        v_r + v_l &= \frac{2 v_y}{\sin\theta} \\
        v_r - v_l &= v_\theta w
    \end{split}
\end{equation}

\begin{equation}
    \begin{split}
        v_r &= \frac{1}{2}\left( \frac{2 v_x}{\cos\theta} + v_\theta w\right) \\
        v_l &= \frac{1}{2}\left( \frac{2 v_x}{\cos\theta} - v_\theta w\right)
    \end{split}
\end{equation}

\begin{equation}
    \begin{split}
        v_r &= \frac{1}{2}\left( \frac{2 v_y}{\sin\theta} + v_\theta w\right) \\
        v_l &= \frac{1}{2}\left( \frac{2 v_y}{\sin\theta} - v_\theta w\right)
    \end{split}
\end{equation}

\begin{equation}
    h(x,y,\theta, v_x, v_y, v_\theta) = 
    \begin{cases}
        \text{range} &= \sqrt{(x_a - x)^2 + (y_a-y)^2}\\
        \text{right} &= \frac{1}{2}\left( \frac{2 v_x}{\cos\theta} + v_\theta w\right) \\
        \text{left} &= \frac{1}{2}\left( \frac{2 v_x}{\cos\theta} - v_\theta w\right) \\
        \text{yaw} &= \gamma + \theta
      \end{cases}
\end{equation}

% \subsubsection{Process model}

% \begin{equation}
%     \begin{split}
%         \alpha &= \frac{r-l}{w} \\
%         R &= \frac{l}{\alpha} = \frac{lw}{r-l}\\
%     \end{split}
% \end{equation}

% \begin{equation}
%     \begin{bmatrix}
%         \hat{x} \\ \hat{y} \\ \hat{\theta} \\
%         \hat{v}_x \\ \hat{v}_y \\ \hat{v}_\theta \\
%         \hat{\gamma}
%     \end{bmatrix}
%     =     
%     \begin{bmatrix}
%         x + \hat{v}_x \\ y + \hat{v}_y \\ \theta + \hat{v}_\theta \\
%         (R+w/2)(\sin{(\theta + \alpha)} - \sin{\theta}) \\(R+w/2)(-\cos{(\theta + \alpha)} + \cos{\theta})\\ v^c_\theta \\
%         \gamma
%     \end{bmatrix}
% \end{equation}

% \begin{equation}
%     \begin{bmatrix}
%         \hat{x} \\ \hat{y} \\ \hat{\theta} \\
%         \hat{v}_x \\ \hat{v}_y \\ \hat{v}_\theta \\
%         \hat{\gamma}
%     \end{bmatrix}
%     =     
%     \begin{bmatrix}
%         x + \hat{v}_x \\ y + \hat{v}_y \\ \theta + \hat{v}_\theta \\
%         l \cos(\theta) \\ l \sin(\theta) \\ 0 \\
%         \gamma
%     \end{bmatrix}
% \end{equation}

\section{Differential}

\begin{equation}
    \frac{\partial f_1}{\partial x} = 1 \qquad
    \frac{\partial f_1}{\partial y} = 0 \qquad
    \frac{\partial f_1}{\partial \theta} = 0 \qquad
    \frac{\partial f_1}{\partial v_x} = 1 \qquad
    \frac{\partial f_1}{\partial v_y} = 0 \qquad
    \frac{\partial f_1}{\partial v_\theta} = 0 \qquad
    \frac{\partial f_1}{\partial \gamma} = 0 \qquad
\end{equation}

\begin{equation}
    \frac{\partial f_2}{\partial x} = 0 \qquad
    \frac{\partial f_2}{\partial y} = 1 \qquad
    \frac{\partial f_2}{\partial \theta} = 0 \qquad
    \frac{\partial f_2}{\partial v_x} = 0 \qquad
    \frac{\partial f_2}{\partial v_y} = 1 \qquad
    \frac{\partial f_2}{\partial v_\theta} = 0 \qquad
    \frac{\partial f_2}{\partial \gamma} = 0 \qquad
\end{equation}

\begin{equation}
    \frac{\partial f_3}{\partial x} = 0 \qquad
    \frac{\partial f_3}{\partial y} = 0 \qquad
    \frac{\partial f_3}{\partial \theta} = 1 \qquad
    \frac{\partial f_3}{\partial v_x} = 0 \qquad
    \frac{\partial f_3}{\partial v_y} = 0 \qquad
    \frac{\partial f_3}{\partial v_\theta} = 1 \qquad
    \frac{\partial f_3}{\partial \gamma} = 0 \qquad
\end{equation}

\begin{equation}
    \begin{split}
    \frac{\partial f_4}{\partial x} = 0 \qquad
    \frac{\partial f_4}{\partial y} = 0 \qquad
    \frac{\partial f_4}{\partial \theta} = -a^c_x\sin{\theta} + a^c_y\cos{\theta}\\
    \frac{\partial f_4}{\partial v_x} = 1 \qquad
    \frac{\partial f_4}{\partial v_y} = 0 \qquad
    \frac{\partial f_4}{\partial v_\theta} = 0 \qquad
    \frac{\partial f_4}{\partial \gamma} = 0 \qquad
\end{split}
\end{equation}

\begin{equation}
    \begin{split}
        \frac{\partial f_5}{\partial x} = 0 \qquad
        \frac{\partial f_5}{\partial y} = 0 \qquad
        \frac{\partial f_5}{\partial \theta} = a^c_x\cos{\theta} - a^c_y\sin{\theta}\\
        \frac{\partial f_5}{\partial v_x} = 0 \qquad
        \frac{\partial f_5}{\partial v_y} = 1 \qquad
        \frac{\partial f_5}{\partial v_\theta} = 0 \qquad
        \frac{\partial f_5}{\partial \gamma} = 0 \qquad
    \end{split}
\end{equation}

\begin{equation}
    \frac{\partial f_6}{\partial x} = 0 \qquad
    \frac{\partial f_6}{\partial y} = 0 \qquad
    \frac{\partial f_6}{\partial \theta} = 0 \qquad
    \frac{\partial f_6}{\partial v_x} = 0 \qquad
    \frac{\partial f_6}{\partial v_y} = 0 \qquad
    \frac{\partial f_6}{\partial v_\theta} = 0 \qquad
    \frac{\partial f_6}{\partial \gamma} = 0 \qquad
\end{equation}

\begin{equation}
    \frac{\partial f_7}{\partial x} = 0 \qquad
    \frac{\partial f_7}{\partial y} = 0 \qquad
    \frac{\partial f_7}{\partial \theta} = 0 \qquad
    \frac{\partial f_7}{\partial v_x} = 0 \qquad
    \frac{\partial f_7}{\partial v_y} = 0 \qquad
    \frac{\partial f_7}{\partial v_\theta} = 0 \qquad
    \frac{\partial f_7}{\partial \gamma} = 0 \qquad
\end{equation}


\begin{equation}
    \frac{\partial f_1}{\partial a^c_x} = 0 \qquad
    \frac{\partial f_1}{\partial a^c_y} = 0 \qquad
    \frac{\partial f_1}{\partial v^c_\theta} = 0
\end{equation}

\begin{equation}
    \frac{\partial f_2}{\partial a^c_x} = 0 \qquad
    \frac{\partial f_2}{\partial a^c_y} = 0 \qquad
    \frac{\partial f_2}{\partial v^c_\theta} = 0
\end{equation}

\begin{equation}
    \frac{\partial f_3}{\partial a^c_x} = 0 \qquad
    \frac{\partial f_3}{\partial a^c_y} = 0 \qquad
    \frac{\partial f_3}{\partial v^c_\theta} = 0
\end{equation}

\begin{equation}
    \frac{\partial f_4}{\partial a^c_x} = \cos \theta \qquad
    \frac{\partial f_4}{\partial a^c_y} = \sin \theta \qquad
    \frac{\partial f_4}{\partial v^c_\theta} = 0
\end{equation}

\begin{equation}
    \frac{\partial f_5}{\partial a^c_x} = \sin \theta \qquad
    \frac{\partial f_5}{\partial a^c_y} = \cos \theta \qquad
    \frac{\partial f_5}{\partial v^c_\theta} = 0
\end{equation}

\begin{equation}
    \frac{\partial f_6}{\partial a^c_x} = 0 \qquad
    \frac{\partial f_6}{\partial a^c_y} = 0 \qquad
    \frac{\partial f_6}{\partial v^c_\theta} = 1
\end{equation}

\begin{equation}
    \frac{\partial f_7}{\partial a^c_x} = 0 \qquad
    \frac{\partial f_7}{\partial a^c_y} = 0 \qquad
    \frac{\partial f_7}{\partial v^c_\theta} = 0
\end{equation}

\end{document}