\documentclass[oneside, 12pt, a4paper]{book}

\usepackage[utf8]{inputenc}
\usepackage[english]{babel}

\usepackage{amsmath}

\providecommand{\main}{.}

\begin{document}
\chapter{EKF}

\section{Prediction}
\begin{equation}
    \begin{split}
        \bar{\mu}_t &= g(\mu_{t-1}, u_t) \\
        \bar{\Sigma}_t &= G_t \Sigma_{t-1} G_t^T + R_t = G_t \Sigma_{t-1} G_t^T + V_t \Sigma_{control} V_t^T 
    \end{split}
\end{equation}

\begin{equation}
    \begin{split}
    \mu_t &= \begin{bmatrix} x & y & \theta \end{bmatrix}^T\\
    u_t &= \begin{bmatrix}l & r \end{bmatrix}^T\\
    \end{split}
\end{equation}

\begin{equation}
    \begin{split}
        \alpha &= \frac{r-l}{w} \\
        R &= \frac{l}{\alpha} = \frac{lw}{r-l}\\
    \end{split}
\end{equation}

$r \neq l$:
\begin{equation}
    g(\mu, u) = 
    \begin{bmatrix}
        x \\ y \\ \theta
    \end{bmatrix}
    +
    \begin{bmatrix}
        (R+w/2)(\sin{(\theta + \alpha)} - \sin{\theta}) \\
        (R+w/2)(-\cos{(\theta + \alpha)} + \cos{\theta}) \\
        \alpha \\
    \end{bmatrix}\\
\end{equation}

$r = l$:
\begin{equation}
    g(\mu, u) = 
    \begin{bmatrix}
        x \\ y \\ \theta
    \end{bmatrix}
    +
    \begin{bmatrix}
        l \cos(\theta) \\
        l \sin(\theta) \\
        0 \\
    \end{bmatrix}\\
\end{equation}

\begin{equation}
    \begin{split}
        G &= \frac{\partial g}{\partial state} \\
    \end{split}
\end{equation}

\begin{equation}
    \frac{\partial g_1}{\partial x} = 1 \qquad
    \frac{\partial g_1}{\partial y} = 0 \qquad
    \frac{\partial g_1}{\partial \theta} = (R+w/2)(\cos{(\theta + \alpha)} - \cos{\theta}) = M
\end{equation}

\begin{equation}
    \frac{\partial g_2}{\partial x} = 0 \qquad
    \frac{\partial g_2}{\partial y} = 1 \qquad
    \frac{\partial g_2}{\partial \theta} = (R+w/2)(\sin{(\theta + \alpha)} - \sin{\theta}) = N
\end{equation}

\begin{equation}
    \frac{\partial g_3}{\partial x} = 0 \qquad
    \frac{\partial g_3}{\partial y} = 0 \qquad
    \frac{\partial g_3}{\partial \theta} = 1
\end{equation}

$l = r$:
\begin{equation}
    \begin{split}
        M &= -l\sin{\theta}\\
        N &= l\cos{\theta}  
    \end{split}
\end{equation}

\begin{equation}
    \frac{\partial g}{\partial state} = \begin{bmatrix}
        1 & 0 & M \\
        0 & 1 & N \\
        0 & 0 & 1 \\ 
    \end{bmatrix}\\
\end{equation}


r != l:

\begin{equation}
    \begin{split}
        A &= \frac{\partial g_1}{\partial l} = \frac{wr}{(r-l)^2}(\sin(\theta + \alpha) - \sin{\theta}) - \frac{r+l}{2(r-l)}\cos(\theta + \alpha)\\
        B &= \frac{\partial g_2}{\partial l} = \frac{wr}{(r-l)^2}(-\cos(\theta + \alpha) + \cos{\theta}) - \frac{r+l}{2(r-l)}\sin(\theta + \alpha)\\
        C &= \frac{\partial g_3}{\partial l} = \frac{-1}{w}
    \end{split}
\end{equation}

\begin{equation}
    \begin{split}
        D &= \frac{\partial g_1}{\partial r} = \frac{-wl}{(r-l)^2}(\sin(\theta + \alpha) - \sin{\theta}) + \frac{r+l}{2(r-l)}\cos(\theta + \alpha)\\
        E &= \frac{\partial g_2}{\partial r} = \frac{-wl}{(r-l)^2}(-\cos(\theta + \alpha) + \cos{\theta}) + \frac{r+l}{2(r-l)}\sin(\theta + \alpha)\\
        F &= \frac{\partial g_3}{\partial r} = \frac{1}{w}
    \end{split}
\end{equation}

r = l:

\begin{equation}
    \begin{split}
        A &= \frac{1}{2}(\cos\theta+\frac{l}{w}\sin\theta)\\
        B &= \frac{1}{2}(\sin\theta-\frac{l}{w}\cos\theta)\\
        C &= \frac{-1}{w}
    \end{split}
\end{equation}

\begin{equation}
    \begin{split}
        D &= \frac{1}{2}(\cos\theta - \frac{l}{w}\sin\theta)\\
        E &= \frac{1}{2}(\sin\theta + \frac{l}{w}\cos\theta)\\
        F &= \frac{\partial g_3}{\partial r} = \frac{1}{w}
    \end{split}
\end{equation}

\begin{equation}
    \begin{split}
        V^T = \begin{bmatrix}
            A & B & C \\
            D & E & F
        \end{bmatrix}
    \end{split}
\end{equation}

\begin{equation}
    \begin{split}
        &G_t \Sigma_{t-1} G_t^T \\
        &= \begin{bmatrix}
            1 & 0 & g_{02} \\
            0 & 1 & g_{12} \\
            0 & 0 & 1 \\ 
        \end{bmatrix}
        \begin{bmatrix}
            s_{00} & s_{01} & s_{02}\\
            s_{10} & s_{11} & s_{12}\\
            s_{20} & s_{21} & s_{22}\\ 
        \end{bmatrix}
        \begin{bmatrix}
            1 & 0 & 0\\
            0 & 1 & 0\\
            g_{02} & g_{12} & 1\\ 
        \end{bmatrix}\\
        &= 
        \begin{bmatrix}
            s_{00}+g_{02}s_{20} & s_{01} + g_{02}s_{21} & s_{02} + g_{02}s_{22}\\
            s_{10} + g_{12}s_{20} & s_{11} + g_{12}s_{21} & s_{12} + g_{12}s_{22}\\
            s_{20} & s_{21} & s_{22}\\
        \end{bmatrix}
        \begin{bmatrix}
            1 & 0 & 0\\
            0 & 1 & 0\\
            g_{02} & g_{12} & 1\\ 
        \end{bmatrix}\\
        &= \begin{bmatrix}
            s_{00}+ g_{02}s_{20} + g_{02}s_{02} + g_{02}^2s_{22}& s_{01} + g_{02}s_{21} + g_{12}s_{02} + g_{02}g_{12}s_{22}& s_{02} + g_{02}s_{22}\\
            s_{10} + g_{12}s_{20} + g_{02}s_{12} + g_{02}g_{12}s_{22} & s_{11} + g_{12}s_{21} + g_{12}s_{12} + g_{12}^2s_{22}& s_{12} + g_{12}s_{22}\\
            s_{20} + g_{02}s_{22} & s_{21} + g_{12}s_{22} & s_{22}\\
        \end{bmatrix}\\
        &= \begin{bmatrix}
            s_{00}+ 2g_{02}s_{02} + g_{02}^2s_{22} & s_{01} + g_{02}s_{12} + g_{12}s_{02} + g_{02}g_{12}s_{22} & s_{02} + g_{02}s_{22}\\
            s_{01} + g_{02}s_{12} + g_{12}s_{02} + g_{02}g_{12}s_{22} & s_{11} + 2g_{12}s_{12} + g_{12}^2s_{22}& s_{12} + g_{12}s_{22}\\
            s_{02} + g_{02}s_{22} & s_{12} + g_{12}s_{22} & s_{22}\\
        \end{bmatrix}
    \end{split}
\end{equation}

\begin{equation}
    \begin{split}
        R^T &= V \Sigma_{control} V^T \\
        &=\begin{bmatrix}
            V_{00} & V_{01}\\
            V_{10} & V_{11}\\
            V_{20} & V_{21}\\
        \end{bmatrix}
        \begin{bmatrix}
            A & 0\\
            0 & B
        \end{bmatrix}
        \begin{bmatrix}
            V_{00} & V_{10} & V_{20} \\
            V_{01} & V_{11} & V_{21}
        \end{bmatrix}\\
        &=\begin{bmatrix}
            V_{00}A^2 & V_{01}B^2\\
            V_{10}A^2 & V_{11}B^2\\
            V_{20}A^2 & V_{21}B^2\\
        \end{bmatrix}
        \begin{bmatrix}
            V_{00} & V_{10} & V_{20}\\
            V_{01} & V_{11} & V_{21}
        \end{bmatrix}\\
        &= \begin{bmatrix}
            V_{00}^2A^2 + V_{01}^2B^2 & V_{00}V_{10}A^2 + V_{01}V_{11}B^2 & V_{00}V_{20}A^2 + V_{01}V_{21}B^2 \\
            V_{10}V_{00}A^2 + V_{11}V_{01}B^2 & V_{10}^2A^2 + V_{11}^2B^2 &V_{10}V_{20}A^2 + V_{11}V_{21}B^2 \\
            V_{20}V_{00}A^2 + V_{21}V_{01}B^2 & V_{20}V_{10}A^2 + V_{21}V_{11}B^2 & V_{20}^2A^2 + V_{21}^2B^2 \\
        \end{bmatrix}
    \end{split}
\end{equation}

\section{Correction}

\begin{equation}
    h(x,y,\theta, x_1, y_1) = 
    \begin{cases}
        r = \sqrt{(x_1 - x_l)^2 + (y_1-y_l)^2} = \sqrt{\Delta x_1^2 + \Delta y_1^2}\\
        \theta' = \theta
      \end{cases}
\end{equation}

\begin{equation}
    \begin{split}
        H &= \frac{\partial h}{\partial state}\\
        &= 
        \begin{bmatrix}
            \frac{\partial r}{\partial x} & \frac{\partial r}{\partial y} & \frac{\partial r}{\partial \theta}\\
            \frac{\partial \theta'}{\partial x} & \frac{\partial \theta'}{\partial y} & \frac{\partial \theta'}{\partial \theta}
        \end{bmatrix}\\
        &=
        \begin{bmatrix}
            \frac{-\Delta x}{r} & \frac{-\Delta y}{r} & \frac{d}{r} (\Delta x\sin\theta - \Delta y\cos\theta) \\
            0 & 0 & 1
        \end{bmatrix}\\
        &=
        \begin{bmatrix}
            H_{00} & H_{01} & H_{02} \\
            0 & 0 & 1
        \end{bmatrix}
    \end{split}
\end{equation}

\begin{equation}
    \begin{split}
        K_t &= \bar{\Sigma}_t H_t^T(H_t \bar{\Sigma}_t H_t^T + Q)^{-1} \\ 
    \end{split}
\end{equation}

\begin{equation}
    \begin{split}
        \bar{\Sigma}_t H_t^T &= 
        \begin{bmatrix}
            s_{00} & s_{01} & s_{02}\\
            s_{10} & s_{11} & s_{12}\\
            s_{20} & s_{21} & s_{22}\\ 
        \end{bmatrix}
        \begin{bmatrix}
            H_{00} & H_{10}\\
            H_{01} & H_{11}\\ 
            H_{02} & H_{12}\\
        \end{bmatrix}\\
        &= 
        \begin{bmatrix}
            M_{00} & M_{01}\\
            M_{10} & M_{11}\\ 
            M_{20} & M_{21}\\
        \end{bmatrix}
    \end{split}
\end{equation}

\begin{equation}
    \begin{split}
        M_{00} &= s_{00}H_{00} + s_{01}H_{01} + s_{02}H_{02} \\
        M_{01} &= s_{00}H_{10} + s_{01}H_{11} + s_{02}H_{22} \\
        M_{10} &= s_{10}H_{00} + s_{11}H_{01} + s_{12}H_{02} \\
        M_{11} &= s_{10}H_{10} + s_{11}H_{11} + s_{12}H_{22} \\
        M_{20} &= s_{20}H_{00} + s_{21}H_{01} + s_{22}H_{02} \\
        M_{21} &= s_{20}H_{10} + s_{21}H_{11} + s_{22}H_{22} \\
    \end{split}
\end{equation}

\begin{equation}
    \begin{split}
        H_t \bar{\Sigma}_t H_t^T &=
        \begin{bmatrix}
            H_{00} & H_{01} & H_{02} \\
            H_{10} & H_{11} & H_{12}
        \end{bmatrix}
        \begin{bmatrix}
            M_{00} & M_{01}\\
            M_{10} & M_{11}\\ 
            M_{20} & M_{21}\\
        \end{bmatrix}\\
        &= 
        \begin{bmatrix}
            T_{00} & T_{01}\\
            T_{10} & T_{11}\\ 
        \end{bmatrix}
    \end{split}
\end{equation}

\begin{equation}
    \begin{split}
        T_{00} &= H_{00}M_{00} + H_{01}M_{10} + H_{02}M_{20} \\
        T_{11} &= H_{10}M_{01} + H_{11}M_{11} + H_{12}M_{21} \\
        T_{01} &= H_{00}M_{01} + H_{01}M_{11} + H_{02}M_{21} \\
        T_{10} &= H_{10}M_{00} + H_{11}M_{10} + H_{12}M_{20}
    \end{split}
\end{equation}

\begin{equation}
    \begin{split}
        A = H_t \bar{\Sigma}_t H_t^T + Q
        &= 
        \begin{bmatrix}
            T_{00} & T_{01}\\
            T_{10} & T_{11}\\ 
        \end{bmatrix}
        +
        \begin{bmatrix}
            Q_{00} & Q_{01}\\
            Q_{10} & Q_{11}\\ 
        \end{bmatrix}\\
        &=
        \begin{bmatrix}
            A_{00} & A_{01}\\
            A_{10} & A_{11}\\ 
        \end{bmatrix}
    \end{split}
\end{equation}

\begin{equation}
    {det}(A) = A_{00}A_{11} - A_{10}A_{01}
\end{equation}

\begin{equation}
    \begin{split}
    A^{-1} &= \frac{1}{det(A)} 
    \begin{bmatrix}
        A_{11} & -A_{01}\\
        -A_{10} & A_{00}\\ 
    \end{bmatrix}\\
    &=
    \begin{bmatrix}
        B_{00} & B_{01}\\
        B_{10} & B_{11}\\ 
    \end{bmatrix}
    \end{split}
\end{equation}


\begin{equation}
    \begin{split}
        K_t &= \bar{\Sigma}_t H_t^T(H_t \bar{\Sigma}_t H_t^T + Q)^{-1} \\ 
        &=
        \begin{bmatrix}
            M_{00} & M_{01}\\
            M_{10} & M_{11}\\ 
            M_{20} & M_{21}\\
        \end{bmatrix} 
        \begin{bmatrix}
            B_{00} & B_{01}\\
            B_{10} & B_{11}\\ 
        \end{bmatrix}\\
        &=
        \begin{bmatrix}
            K_{00} & K_{01}\\
            K_{10} & K_{11}\\ 
            K_{20} & K_{21}\\
        \end{bmatrix} 
    \end{split}
\end{equation}

\begin{equation}
    \begin{split}
        K_{00} &= M_{00}B_{00} + M_{01}B_{10} \\
        K_{01} &= M_{00}B_{01} + M_{01}B_{11} \\
        K_{10} &= M_{10}B_{00} + M_{11}B_{10} \\
        K_{11} &= M_{10}B_{01} + M_{11}B_{11} \\
        K_{20} &= M_{20}B_{00} + M_{21}B_{10} \\
        K_{21} &= M_{20}B_{01} + M_{21}B_{11}
    \end{split}
\end{equation}

\begin{equation}
    \begin{split}
        \mu_t &= \bar{\mu}_t + K_t(Z_t - h(\bar{\mu}_t))\\
        \Sigma_t&= (I-K_tH_t)\bar{\Sigma}_t\\
    \end{split}
\end{equation}

\begin{equation}
    \begin{split}
        \mu_t &= \bar{\mu}_t + K_t(Z_t - h(\bar{\mu}_t))\\
        &= 
        \begin{bmatrix}
            x\\
            y\\ 
            \theta\\
        \end{bmatrix} 
        +
        \begin{bmatrix}
            K_{00} & K_{01}\\
            K_{10} & K_{11}\\ 
            K_{20} & K_{21}\\
        \end{bmatrix} 
        \left(
            \begin{bmatrix}
                Z_{0}\\
                Z_{1}\\ 
            \end{bmatrix}
            -
            \begin{bmatrix}
                h_{0}\\
                h_{1}\\ 
            \end{bmatrix} 
        \right)\\
        &=
        \begin{bmatrix}
            x\\
            y\\ 
            \theta\\
        \end{bmatrix} 
        +
        \begin{bmatrix}
            K_{00} & K_{01}\\
            K_{10} & K_{11}\\ 
            K_{20} & K_{21}\\
        \end{bmatrix} 
        \begin{bmatrix}
            D_{0}\\
            D_{1}\\ 
        \end{bmatrix}\\
        &=
        \begin{bmatrix}
            x + K_{00}D_0 + K_{01}D_1\\
            y + K_{10}D_0 + K_{11}D_1\\ 
            \theta + K_{20}D_0 + K_{21}D_1\\
        \end{bmatrix} 
    \end{split}
\end{equation}

\begin{equation}
    \begin{split}
        K_tH_t &=
        \begin{bmatrix}
            K_{00} & K_{01}\\
            K_{10} & K_{11}\\ 
            K_{20} & K_{21}\\
        \end{bmatrix}
        \begin{bmatrix}
            H_{00} & H_{01} & H_{02} \\
            H_{10} & H_{11} & H_{12}
        \end{bmatrix}\\
        &=
        \begin{bmatrix}
            A_{00} & A_{01} & A_{02}\\
            A_{10} & A_{11} & A_{12}\\ 
            A_{20} & A_{21} & A_{22}\\
        \end{bmatrix}
    \end{split}
\end{equation}

\begin{equation}
    \begin{split}
        I - K_tH_t &=
        \begin{bmatrix}
            B_{00} & B_{01} & B_{02}\\
            B_{10} & B_{11} & B_{12}\\ 
            B_{20} & B_{21} & B_{22}\\
        \end{bmatrix}
    \end{split}
\end{equation}

\begin{equation}
    \begin{split}
        (I - K_tH_t)\bar{\Sigma}_t &=
        \begin{bmatrix}
            B_{00} & B_{01} & B_{02}\\
            B_{10} & B_{11} & B_{12}\\ 
            B_{20} & B_{21} & B_{22}\\
        \end{bmatrix}
        \begin{bmatrix}
            c_{00} & c_{01} & c_{02}\\
            c_{10} & c_{11} & c_{12}\\ 
            c_{20} & c_{21} & c_{22}\\
        \end{bmatrix}
    \end{split}
\end{equation}

\end{document}